theories/Core/Semantic/Evaluation/Definitions.v
@@ -5,6 +5,7 @@ Import Domain_Notations.
 
 Reserved Notation "'⟦' M '⟧' ρ '↘' r" (in custom judg at level 80, M custom exp at level 99, ρ custom domain at level 99, r custom domain at level 99).
 Reserved Notation "'$|' m '&' n '|↘' r" (in custom judg at level 80, m custom domain at level 99, n custom domain at level 99, r custom domain at level 99).
+Reserved Notation "'rec' m '⟦return' A | 'zero' -> MZ | 'succ' -> MS 'end⟧' ρ '↘' r" (in custom judg at level 80, m custom domain at level 99, A custom exp at level 99, MZ custom exp at level 99, MS custom exp at level 99, ρ custom domain at level 99, r custom domain at level 99).
 Reserved Notation "'⟦' σ '⟧s' ρ '↘' ρσ" (in custom judg at level 80, σ custom exp at level 99, ρ custom domain at level 99, ρσ custom domain at level 99).
 (** Since environments are lists and not functions, we need to explicitly define lookups *)
 Reserved Notation "'#|' ρ '[' n ']' '|↘' m" (in custom judg at level 80, ρ custom domain, n constr at level 0, m custom domain at level 99). 
@@ -39,6 +40,17 @@ Inductive eval_exp {P : PtsSig} : exp P -> env P -> domain P -> Prop :=
      {{ ⟦ N ⟧ ρ ↘ n }} ->
      {{ $| m & n |↘ m' }} ->
      {{ ⟦ M N ⟧ ρ ↘ m' }} )
+| eval_exp_nat :
+  `( {{ ⟦ ℕ ⟧ ρ ↘ ℕ }} )
+| eval_exp_zero :
+  `( {{ ⟦ zero ⟧ ρ ↘ zero }} )
+| eval_exp_succ :
+  `( {{ ⟦ M ⟧ ρ ↘ m }} ->
+     {{ ⟦ succ M ⟧ ρ ↘ succ m }} )
+| eval_exp_natrec :
+  `( {{ ⟦ M ⟧ ρ ↘ m }} ->
+     {{ rec m ⟦return A | zero -> MZ | succ -> MS end⟧ ρ ↘ r }} ->
+     {{ ⟦ rec M return A | zero -> MZ | succ -> MS end ⟧ ρ ↘ r }} )
 | eval_exp_sub :
   `( {{ ⟦ σ ⟧s ρ ↘ ρ' }} ->
      {{ ⟦ M ⟧ ρ' ↘ m }} ->
@@ -54,6 +66,19 @@ with eval_app {P : PtsSig} : domain P -> domain P -> domain P -> Prop :=
       {{ ⟦ B ⟧ ρ ↦ n ↘ b }} ->
       {{ $| ⇑ (Π r a ρ B) m & n |↘ ⇑ b (m (⇓ a n)) }} )
 where "'$|' m '&' n '|↘' m'" := (eval_app m n m') (in custom judg)
+with eval_natrec {P : PtsSig} : exp P -> exp P -> exp P -> domain P -> env P -> domain P -> Prop :=
+| eval_natrec_zero :
+  `( {{ ⟦ MZ ⟧ ρ ↘ mz }} ->
+     {{ rec zero ⟦return A | zero -> MZ | succ -> MS end⟧ ρ ↘ mz }} )
+| eval_natrec_succ :
+  `( {{ rec b ⟦return A | zero -> MZ | succ -> MS end⟧ ρ ↘ r }} ->
+     {{ ⟦ MS ⟧ (ρ ↦ b) ↦ r ↘ ms }} ->
+     {{ rec succ b ⟦return A | zero -> MZ | succ -> MS end⟧ ρ ↘ ms }} )
+| eval_natrec_neut :
+  `( {{ ⟦ MZ ⟧ ρ ↘ mz }} ->
+     {{ ⟦ A ⟧ ρ ↦ ⇑ b m ↘ a }} ->
+     {{ rec ⇑ b m ⟦return A | zero -> MZ | succ -> MS end⟧ ρ ↘ ⇑ a (rec m under ρ return A | zero -> mz | succ -> MS end) }} )
+where "'rec' m '⟦return' A | 'zero' -> MZ | 'succ' -> MS 'end⟧' ρ '↘' r" := (eval_natrec A MZ MS m ρ r) (in custom judg)
 with eval_sub {P : PtsSig} : sub P -> env P -> env P -> Prop :=
 | eval_sub_id :
   `( {{ ⟦ Id ⟧s ρ ↘ ρ }} )
@@ -72,11 +97,13 @@ where "'⟦' σ '⟧s' ρ '↘' ρσ" := (eval_sub σ ρ ρσ) (in custom judg)
 
 Scheme eval_exp_mut_ind := Induction for eval_exp Sort Prop
 with eval_app_mut_ind := Induction for eval_app Sort Prop
+with eval_natrec_mut_ind := Induction for eval_natrec Sort Prop
 with eval_sub_mut_ind := Induction for eval_sub Sort Prop.
 Combined Scheme eval_mut_ind from
   eval_exp_mut_ind,
   eval_app_mut_ind,
+  eval_natrec_mut_ind,
   eval_sub_mut_ind.
 
 #[export]
-Hint Constructors eval_exp eval_app eval_sub : mcpts.
+Hint Constructors eval_exp eval_app eval_natrec eval_sub : mcpts.
